\section{Integrals in QFT}

\subsection{Kinetic operator and a Green Function} \label{integral:kinetic-operator}

This problem is part of
\href{https://arxiv.org/abs/physics/0609191}{MontePython: Implementing Quantum Monte Carlo using Python}.

There is a kinetic operator defined as
$$
G_K \left(\mathbf{R}^\prime, \mathbf{R}, t\right) =
\frac{1}{\left(2\pi\right)^{3N}} \int e^{-i\mathbf{k}\mathbf{R}^\prime} e^{-Dtk^2} e^{-i\mathbf{k}\mathbf{R}} d\mathbf{k}
$$

This integral then is integrated and the following Green function is obtained
$$
G_K \left(\mathbf{R}^\prime, \mathbf{R}, t\right) =
\frac{1}{\left(4\pi Dt\right)^{3N/2}} e^{-\left(\mathbf{R}-\mathbf{R}^\prime\right) / 4Dt}
$$

And as we saw in \hyperref[jackson:problem-1.2]{Jackson problem 1.2}, the Green function we just got is equivalent to
$\delta\left(\mathbf{R} - \mathbf{R}^\prime\right)$.

But coming back to the integral, the trick is to complete the square!
\begin{align*}
G_K \left(\vect{R}^\prime, \vect{R}, t\right) &=
\frac{1}{\left(2\pi\right)^{3N}} \int e^{-i\vect{k}\vect{R}^\prime} e^{-Dtk^2} e^{-i\vect{k}\vect{R}} d\vect{k} \\
&= \frac{1}{\left(2\pi\right)^{3N}} \int e^{-Dtk^2 + -i\vect{k}\cdot\left(\vect{R}-\vect{R}^\prime\right)} d\mathbf{k}
\end{align*}

This last integral has the form $\int e^{ax^2 + bx} dx$, which can be solved as follows,
\begin{align*}
\int e^{ax^2 + bx} dx &= \int \exp\left\{ a\left(x^2 + \frac{b}{a}x\right) \right\} dx \\
&= \int \exp\left\{ a\left(x^2 + \frac{b}{a}x + \left(\frac{b}{2a}\right)^2 - \left(\frac{b}{2a}\right)^2 \right) \right\} dx \\
&= \int \exp\left\{ a\left(x + \frac{b}{2a}\right)^2 - \frac{b^2}{4a} \right\} dx \\
&= e^{-b^2/4a} \int e^{ a\left(x + \frac{b}{2a}\right)^2 } dx
\end{align*}

Now, let's look at $\int e^{ a\left(x + b/2a\right)^2 } dx$.
First, we need to make a transformation.
Let's define $u = x + b/2a$, then $du = dx$, the measure remains invariant (so do the limits of integration), so
$\int e^{ a\left(x + b/2a\right)^2 } dx = \int e^{ au^2 } du$.
Now, if we define $a = -c$, then 

\begin{align*}
\int e^{ a\left(x + b/2a\right)^2 } dx &= \int e^{ au^2 } du \\
&= \int e^{ -cu^2 } du \\
&= \sqrt{ \frac{\pi}{c} } = \sqrt{ \frac{\pi}{-a} } 
\end{align*}

This whole thing works if $a < 0$ but it turns out that this is also valid if $\re{(a)} \leq 0$ but $a \neq 0$.

Putting everything back together,
$$
\int e^{ax^2 + bx} dx = \sqrt{ \frac{\pi}{-a} } e^{-b^2/4a}
$$

Looking back at our original problem, we can chose $a = -Dt$ and $b = i \vect{r}$, where $\vect{r} = \vect{R}-\vect{R}^\prime$.
and so
\begin{align*}
G_K \left(\vect{R}^\prime, \vect{R}, t\right) &=
\frac{1}{\left(2\pi\right)^{3N}} \int e^{-Dtk^2 + -i\vect{k}\cdot\vect{r}} d\mathbf{k} \\
&= \frac{1}{\left(2\pi\right)^{3N}} \int e^{-Dt \left( k^2 + \frac{i\vect{k}}{Dt}\cdot\vect{r} \right)} d\mathbf{k} \\
&= \frac{1}{\left(2\pi\right)^{3N}} \int e^{-Dt \left( k^2 + \frac{i\vect{r}}{Dt}\cdot\vect{k} + \left(\frac{i\vect{r}}{2Dt}\right)^2 - \left(\frac{i\vect{r}}{2Dt}\right)^2 \right)} d\mathbf{k} \\
&= \frac{1}{\left(2\pi\right)^{3N}} \int e^{-Dt \left( k + \frac{i\vect{r}}{2Dt}\right)^2 - \frac{ \vect{r}^2 }{ 4Dt } } d\mathbf{k} \\
&= \frac{1}{\left(2\pi\right)^{3N}} e^{-\vect{r}^2 /4Dt } \int e^{-Dt \left( k + \frac{i\vect{r}}{2Dt}\right)^2 } d\mathbf{k} \\
\end{align*}

Again, since $\int e^{-ax^2} dx = \sqrt{ \frac{\pi}{a} }$,
then
\begin{align*}
\int e^{-Dt \left( k + \frac{i\vect{r}}{2Dt}\right)^2 } dk &= \sqrt{ \frac{\pi}{Dt} }
\end{align*}

Thus,
\begin{align*}
G_K \left(\vect{R}^\prime, \vect{R}, t\right) &=
\frac{1}{\left(2\pi\right)^{3N}} e^{-\vect{r}^2 /4Dt } \int e^{-Dt \left( k + \frac{i\vect{r}}{2Dt}\right)^2 } d\mathbf{k} \\
&= \frac{1}{\left(2\pi\right)^{3N}} e^{-\vect{r}^2 /4Dt } \left( \sqrt{ \frac{\pi}{Dt} } \right)^{3N} \\
&= \frac{1}{\left(4\pi^2\right)^{3N/2}} \frac{\pi^{3N/2}}{(Dt)^{3N/2}} e^{-\vect{r}^2 /4Dt } \\
&= \frac{1}{\left(4\pi Dt\right)^{3N/2}} e^{-\left(\vect{R} - \vect{R}^\prime\right)^2 /4Dt }
\end{align*}



%%%%%%%%%%%%%%%%%%%%%%%%%%%%%%%%%%%%%%%%%%%%%%%%%%%%%%%%%%%%%%%%%%%%%%%%%%%%%%%%%%%%%%%%%%%%%%%%%%%%%%%%%

\subsection{Klein-gordon Non-relativistic Amplitude} \label{ps-kg:nonrelativistic-propagator}

The following integral comes from Peskin and schroeder Section 2.1
\begin{align}
& \int \frac{d^3p}{(2\pi)^3} \, e^{-i(\vect{p}^2/2m)t} e^{i\vect{p}\cdot(\vect{x}-\vect{x}_0)} %\label{kg:nonrelativistic-03} \\
&= \left( \frac{m}{2\pi i t} \right)^{3/2} e^{im (\vect{x}-\vect{x}_0)^2 /2t} %\label{kg:nonrelativistic-04}
\end{align}

This integral follows the same procedure as \ref{integral:kinetic-operator}.

Here we have $a = -\frac{it}{2m}$ and $b = i(\vect{x}-\vect{x_0})$.
Since $\re{a} = -t/2m \leq 0$ and $a\neq 0$ when $t\neq 0$ oru solution is valid for $t\neq 0$.
Then

$$
\sqrt{ \frac{\pi}{-a} } = \sqrt{ \frac{2\pi m}{it} }
$$

and
\begin{align*}
-\frac{b^2}{4a} &= \frac{2m \left(\vect{x}-\vect{x}_0\right)^2}{-4it} \\
&= \frac{im \left(\vect{x}-\vect{x}_0\right)^2}{2t}
\end{align*}

So the solution is
\begin{align*}
& \frac{1}{(2\pi)^3} \left( \frac{2\pi m}{it} \right)^{3/2} e^{\frac{im \left(\vect{x}-\vect{x}_0\right)^2}{2t}} \\
&= \left( \frac{m}{2\pi it} \right)^{3/2} e^{im \left(\vect{x}-\vect{x}_0\right)^2 /2t}
\end{align*}