\chapter{Intro to QFT}

\section{Inivitation}

\subsection{Polarization Vectors}

In the invitation, we are presented with the polarization vector $\epsilon^\mu = (0, 1, i, 0)$.

To understand this notation let's go through some examples taken from
\href{https://scholar.harvard.edu/files/schwartz/files/lecture14-polarization.pdf}{Lecture 14: Polarization}.

We say that a plane wave is \textbf{linearly polarized} if there is no phase difference between $E_x$ and $E_y$:
$$
\vect{E}_0 = \left( E_x, E_y, 0 \right)
$$

Then a linearly polarized plane wave in the x direction looks like $\vect{E} = E_0 e^{i(kz-wt)} (1, 0, 0)$.
And a linearly polarized plane wave in the y direction looks like $\vect{E} = E_0 e^{i(kz-wt)} (0, 1, 0)$.

The thing to remember is that we are implicitly only looking at the real part, so a linearly polarized wave in the x
direction is actually $(E_0 \cos(kz-wt), 0, 0)$.
\\

\textbf{Circular polarization} is when the electric field components are one-quarter out of phase ($\pi /2$).
Then the field can be written as,

\begin{align*}
\vect{E}_0 &= \left( E_0, E_0 e^{i\pi/2}, 0 \right) \\
&= \left( E_0, iE_0, 0 \right) \\
&= E_0 \left( e^{i(kz-wt)}, ie^{i(kz-wt)}, 0 \right)
\end{align*}

And since we only care about the real parts,
$$
\vect{E}_0 = \left( cos(kz-wt), -sin(kz-wt), 0 \right)
$$

This is interesting because if you jump to the wikipedia page for "List of trigonometric identities"
and look for the "Shift by one quarter period" table, you'll see that
$$
\sin(\theta + \frac{\pi}{2}) = \cos(\theta)
$$
and
$$
\cos(\theta + \frac{\pi}{2}) = -\cos(\theta)
$$

(A shit by a quarter wavelength is essentially differentiation!)

But here is the catch and the connection with P\&S: we can also get the same result if we have
$$
\vect{E} = E_0 \left( \cos(wt-kz)\hat{x} + \sin(wt-kz)\hat{y} \right)
$$
We can also write is as,
$$
E_0 e^{i(wt - kz)} (0, 1, i, 0)
$$
and remembering that you only care about the real part.
If you do so, you'll end up with terms such as $\cos \hat{x} - \sin \hat{y}$ which just so happen to again be the
a $\sin$ and a $\cos$ (our original plane wave components) shifted by $\pi/2$.




\subsection{Cross Sections}

The next thing we want to document is how to solve the differential cross section (per unit solid angle).
The expression given was

$$
\frac{d\sigma}{d\Omega} = \frac{\alpha^2}{4E_{cm}^{2}} (1 + \cos^2 \theta)
$$

That when integrated gives the total cross section
$$
\sigma_{total} = \frac{4\pi\alpha^2}{3E_{cm}^{2}}
$$

The trick here is to identity $d\Omega = \sin\theta \, d\theta \, d\phi$.
So essentially the problem is to integrate

\begin{align*}
\int d\Omega \, \left( 1 + \cos\theta \right) &=
    \int_{\phi=0}^{2\pi} \int_{\theta=0}^{\pi} \left( 1 + \cos\theta \right) \sin\theta \, d\theta \, d\phi \\
&= \left( \int_{\phi=0}^{2\pi} \int_{\theta=0}^{\pi} \sin\theta \, d\theta \, d\phi \right)
    + \left( \int_{\phi=0}^{2\pi} \int_{\theta=0}^{\pi} \cos\theta \sin\theta \, d\theta \, d\phi \right) \\
&= \left( 4\pi \right) + \left( -\int u^2 du \right) \\
&= \left( 4\pi \right) + \left( -\frac{1}{3} \cos^3 \theta \Big|_{0}^{\pi} du \right) \\
&= \left( 4\pi \right) \left( 2\pi \frac{8}{3} \right) \\
&= \frac{16\pi}{3}
\end{align*}

Note that we did a $u$-substitution in the second integral: $u = \cos\theta$, so $du = -\sin\theta \, d\theta$.







%%%%%%%%%%%%%%%%%%%%%%%%%%%%%%%%%%%%%%%%%%%%%%%%%%%%%%%%%%%%%%%%%%%%%%%%%%%%%%%%%%%%

\section{The Klein-Gordon Field}

\subsection{Klein-Gordon Inconsistensies}

The Schrodinger equation canr readily be abtain treating the energy and momentum as operators.
In quantum mechanics $E = i\partial_t$ and $p = -i\nabla$.
Using the realtionship $E = \frac{p^2}{2}$, we get


$$
i\partial_t \ket{\psi} = -\frac{1}{2m} \nabla^2 \ket{\psi}
$$

Note that we are still in natural units, otherwise there would be an $\hbar$.

The Klein-Gordon equation comes if we instead use $E^2 - p^2 = m^2$,

$$
-\partial_{t}^2 \ket{\psi} + \nabla^2 \ket{\psi} = m^2 \ket{\psi}
$$

And remember that $\partial^2 = \partial_{t}^{2} - \nabla^2$, so there comes $(\partial^2 - m)\psi = 0$ equation.



%%%%%%%%%%%%%%%%%%%%%%%%%%%%%%%%%%%%%%%%%%%%%%%%%%%%%%%%%%%%%%%%%%%%%%%%%%%%%%%
\subsubsection{Klein-Gordon Solution}

One method to solve the equation is to use Fourier transforms.
So we can begin by expressing the wave function $\phi(x,t)$ as a Fourier integral,

$$
\psi(x, t) =
\int \frac{d^4k}{\left(2\pi\right)^4} \tilde{\psi}(k, \omega) e^{-i(k\cdot x - \omega t)}
$$

Here, $\tilde{\psi}(k, \omega)$ is the Fourier transform of $\psi(x, t)$.
One thing that's often missed is the rgument of the exponent: if you look back to examples where we talk about plane waves
(just go back to the previous section), a wave with positive momentum moving in positive direction $x$ has the argument $wt - xk$.
And the convention is to hae such a wave in the Fourier transform.

With this Fourier transofrm in place, we take the Fourier transform of our entire differential equation to reduce
the solution into an algebraic problem.

For example, applying the Fourier transform to the time derivative goes as follows:

\begin{align*}
\mathcal{F}\{ \partial_t \psi \} &=
    \int \frac{d^4k}{(2\pi)^4} \partial_t \psi e^{-i(\vect{k}\cdot\vect{x} - \omega t)}
\rightarrow
\left[
    \begin{alignedat}{2}
        u  &= e^{-i(\vect{k}\cdot\vect{x} - \omega t)}                \quad & v  &= \psi \\
        du &= i\omega e^{-i(\vect{k}\cdot\vect{x} - \omega t)} \, dt  \quad & dv &= \partial_t \psi \, dt
    \end{alignedat}\,
\right] \\
&= \cancelto{0}{ \psi(\vect{x}, t) e^{-i(\vect{k}\cdot\vect{x} - \omega t)} } \Big|_{t=-\infty}^{t=\infty}
    - \int \frac{d^4k}{(2\pi)^4} \psi(\vect{x}, t) \left(i\omega\right) e^{-i(\vect{k}\cdot\vect{x} - \omega t)} \\
&= -i\omega \tilde{\psi} (\vect{k}, \omega)
\end{align*}

We made use of the integration by parts technique ($\int u \, dv = uv - \int v \, du$) to transfer the time derivative
on $\psi$ to the exponent term.

As per the boudnary term, we have a couple words to say: physically, the wave function (or even field) should vanish at infinity.
Mathematically, in order for the Fourier transform to converge to a value the function that is being "transformed", $\psi$,
must be a \textbf{rapidly decreasing function} (a function of \href{https://en.wikipedia.org/wiki/Schwartz_space}{Schwartz space}).

Similarly then,

\begin{align*}
\mathcal{F}\{ \partial_{t}^2 \psi \} &=
    \int \frac{d^4k}{(2\pi)^4} \partial_{t}^{2} \psi e^{-i(\vect{k}\cdot\vect{x} - \omega t)}
\rightarrow
\left[
    \begin{alignedat}{2}
        u  &= e^{-i(\vect{k}\cdot\vect{x} - \omega t)}                \quad & v  &= \partial_t \psi \\
        du &= i\omega e^{-i(\vect{k}\cdot\vect{x} - \omega t)} \, dt  \quad & dv &= \partial_{t}^{2} \psi \, dt
    \end{alignedat}\,
\right] \\
&= \cancelto{0}{ \partial _t \psi(\vect{x}, t) e^{-i(\vect{k}\cdot\vect{x} - \omega t)} } \Big|_{t=-\infty}^{t=\infty}
    - \int \frac{d^4k}{(2\pi)^4} \partial_t \psi(\vect{x}, t) \left(i\omega\right) e^{-i(\vect{k}\cdot\vect{x} - \omega t)} \\
&= -i\omega \mathcal{F}\{ \partial_t \psi \} \\
&= - \omega^2 \tilde{\psi} (\vect{k}, \omega)
\end{align*}

The boundary term again goes to zero here.
We will skip the physical argument and just mention that a rapidly decreasin function also requires all of its derivatives
tend to zero.



For the spatial derivatives, each $\partial_i$ will bring down a factor of $-i k_i$, resulting in a factor of
$- k_{i}^2$ for each $\partial_{i}^{2}$.
And this is something that always triped me up: one may be inclined to write $-k^2$ in the Fourier transform
but that same one ought to remember that $k$ is actually $\vec{k}$ (a vector) and that is why we must
write $-|k|^2$, because we want the [L-2] norm.

But anyways, the Fourier transform of the Laplacian is,

\begin{align*}
\mathcal{F}\{ \nabla \psi \} &=
    \int \frac{d^4k}{(2\pi)^4} \nabla \psi e^{-i(\vect{k}\cdot\vect{x} - \omega t)}
\rightarrow
\left[
    \begin{alignedat}{2}
        u  &= e^{-i(\vect{k}\cdot\vect{x} - \omega t)}                          \quad & v  &= \psi \\
        du &= -i\vect{k} e^{-i(\vect{k}\cdot\vect{x} - \omega t)} \, d\vect{x}  \quad & dv &= \nabla \psi \, d\vect{x}
    \end{alignedat}\,
\right] \\
&= \cancelto{0}{ \psi(\vect{x}, t) e^{-i(\vect{k}\cdot\vect{x} - \omega t)} } \Big|_{\vect{x}=-\infty}^{\vect{x}=\infty}
    - \int \frac{d^4k}{(2\pi)^4} \psi(\vect{x}, t) \left(-i\vect{k}\right) e^{-i(\vect{k}\cdot\vect{x} - \omega t)} \\
&= -i\vect{k} \tilde{\psi} (\vect{k}, \omega)
\end{align*}


and

\begin{align*}
\mathcal{F}\{ \nabla^2 \psi \} &=
    \int \frac{d^4k}{(2\pi)^4} \nabla^2 \psi e^{-i(\vect{k}\cdot\vect{x} - \omega t)}
\rightarrow
\left[
    \begin{alignedat}{2}
        u  &= e^{-i(\vect{k}\cdot\vect{x} - \omega t)}                          \quad & v  &= \nabla \psi \\
        du &= -i\vect{k} e^{-i(\vect{k}\cdot\vect{x} - \omega t)} \, d\vect{x}  \quad & dv &= \nabla^2 \psi \, d\vect{x}
    \end{alignedat}\,
\right] \\
&= \cancelto{0}{ \nabla\psi(\vect{x}, t) e^{-i(\vect{k}\cdot\vect{x} - \omega t)} } \Big|_{\vect{x}=-\infty}^{\vect{x}=\infty}
    - \int \frac{d^4k}{(2\pi)^4} \nabla\psi(\vect{x}, t) \left(-i\vect{k}\right) e^{-i(\vect{k}\cdot\vect{x} - \omega t)} \\
&= -i\vect{k} \mathcal{F}\{ \nabla \psi \} \\
&= - |\vect{k}|^2 \tilde{\psi} (\vect{k}, \omega)
\end{align*}



And since the above must hold throughout all of space, that's where
$$
\left(-\omega^2 + |\vect{k}|^2 + m^2 \right) \tilde{\psi}(\vect{k}, \omega) = 0
$$
comes from!

Now, in order for us to not have a trivial solution, $\psi(\vect{x}, t) = 0$, it must be so that
$\left(-\omega^2 + |\vect{k}|^2 + m^2 \right) = 0$, and so our dispersion relation comes about
$$
\omega^2 = |\vect{k}|^2 + m^2
$$
So $\omega = \pm \sqrt{ |\vect{k}|^2 + m^2 }$.
So essentially any function will do as long as the dispersion relation (momentum conservation) is respected.

A thing that people do, specially since we are talking about Fourier transforms is to define

$$
\psi(\vect{k}, \omega) = A(\vec{k}) \delta\left( \omega - \sqrt{ |\vect{k}|^2 + m^2 }\right) +
    B(\vec{k}) \delta\left( \omega + \sqrt{ |\vect{k}|^2 + m^2 }\right)
$$

Note that $A(\vec{k})$ and $B(\vec{k})$ are arbitrary functions that only depend on $\vect{k}$ since the
Dirac delta functions specifies the value for $\omega$.

With that, we can finally write a solution for the differential equation we started with,

\begin{align*}
\psi(\vect{x}, t) &=
    \int \frac{d^4k}{(2\pi)^4} \left[
        A(\vec{k}) \delta\left( \omega - \sqrt{ |\vect{k}|^2 + m^2 }\right) e^{-i(\vect{k}\cdot\vect{x} -\omega t)} +
        B(\vec{k}) \delta\left( \omega + \sqrt{ |\vect{k}|^2 + m^2 }\right) e^{-i(\vect{k}\cdot\vect{x} -\omega t)}
    \right] \\
&= \int \frac{d^4k}{(2\pi)^4} \left[
    A(\vec{k}) e^{-i(\vect{k}\cdot\vect{x} - \sqrt{ |\vect{k}|^2 + m^2 } t)} +
    B(\vec{k}) e^{-i(\vect{k}\cdot\vect{x} + \sqrt{ |\vect{k}|^2 + m^2 } t)}
\right]
\end{align*}

Hopefully thiis result makes sense: we obtained a family of function as solution and only initial conditions or
boundary conditions will result in a specific sort of function.




%%%%%%%%%%%%%%%%%%%%%%%%%%%%%%%%%%%%%%%%%%%%%%%%%%%%%%%%%%%%%%%%%%%%%%%%%%%%%%%
\subsubsection{Klein-Gordon Negative Density}




%%%%%%%%%%%%%%%%%%%%%%%%%%%%%%%%%%%%%%%%%%%%%%%%%%%%%%%%%%%%%%%%%%%%%%%%%%%%%%%
\subsubsection{A Propagator}

Describes the amplitude for a particle to propagate from one point to another.

With a source $j(\vect{x}, t)$, the Klein-Gordon equation becomes
$$
\left( \partial^2 + m^2 \right) \psi(\vect{x}, t) = j(\vect{x}, t)
$$

In momentum space the equation is
$$
\left( -\omega^2 + |\vect{k}|^2 + m^2 \right) \tilde{\psi}(\vect{k}, \omega) = \tilde{j}(\vect{\vect{k}, \omega})
$$

$$
\tilde{\psi}(\vect{k}, \omega) = \frac{ \tilde{j}(\vect{\vect{k}, \omega}) }{ \omega^2 - |\vect{k}|^2 - m^2 + i\epsilon }
$$

$i\epsilon$ Feynman's prescription.

The propagator $D_F(x-y)$ is the inverse transform of
$\frac{ 1 }{ \omega^2 - |\vect{k}|^2 - m^2 + i\epsilon }$

$$
D_F(x-y) = \int \frac{d^4k}{(2\pi)^4}
    \frac{ e^{-i(\vect{k}\cdot\vect{x} -\omega t)} }{ \omega^2 - |\vect{k}|^2 - m^2 + i\epsilon }
$$