\section{Vector Spaces}

\subsection{Vectors in Function Spaces}


\textbf{Scwarz Inequality}


\begin{align*}
I &= \braket{f - \lambda g | f - \lambda g} \\
&= \left( \bra{f} - \lambda^* \bra{g} \right) \left( \ket{f} - \lambda \ket{g} \right) \\
&= \braket{f|f} - \lambda \braket{f|g} - \lambda^* \braket{g|f} + \lambda^* \lambda \braket{g|g} \\
&= \braket{f|f} + |\lambda|^2 \braket{g|g} - \left( \braket{\lambda g|f} + \braket{f | \lambda g} \right) \\
&= \braket{f|f} + |\lambda|^2 \braket{g|g} - \left( \braket{f | \lambda g}^* + \braket{f | \lambda g} \right) \\
&= |f|^2 + |\lambda|^2 |g|^2 - \left( \braket{f | \lambda g}^* + \braket{f | \lambda g} \right) \\
& \geq 0
\end{align*}

If we were looking at complex numbers, the term in the braces would equal $2\Re(z)$.

\begin{align*}
\partial_{\lambda^*} I &= \partial_{\lambda^*} \left( \bra{f} -\lambda^*\bra{g} \right)\left(\ket{f - \lambda g}\right) \\
&= - \braket{g|f} + \lambda \braket{g|g} = 0
\end{align*}

The above implies that
$$
\lambda = \frac{\braket{g|f}}{\braket{g|g}}
$$

If we plug that in, we have,
\begin{align*}
I &= \braket{f|f} + |\lambda|^2 \braket{g|g} - \braket{\lambda g|f} - \braket{f | \lambda g} \\
&= \braket{f|f} + \frac{\braket{f|g}\braket{g|f}}{\braket{g|g}^2} \braket{g|g}
    - \frac{\braket{f|g}}{\braket{g|g}} \braket{g|f}
    - \frac{\braket{g|f}}{\braket{g|g}} \braket{f | g} \\
&= \braket{f|f} + \frac{\braket{f|g}\braket{g|f}}{\braket{g|g}}
    - \frac{\braket{f|g}}{\braket{g|g}} \braket{g|f}
    - \frac{\braket{g|f}}{\braket{g|g}} \braket{f | g} \\
&= \braket{f|f}
    - \frac{\braket{g|f}}{\braket{g|g}} \braket{f | g} \\
&\geq 0
\end{align*}

So
$$
\braket{f|f} \braket{g|g} \geq \braket{g|f} \braket{f|g} = |\braket{f|g}|^2
$$