\section{Setting the Stage}

\subsection{Euclidean Spaces and Vectors}

\subsubsection{Exercises}

\textbf{1.1.2}

Given $\vec{x}, \vec{y} \in \mathbb{R^n}$,
\begin{align*}
|\vec{x} + \vec{y} |^2 &= (\vec{x} +\vec{y}) (\vec{x} +\vec{y}) \\
&= \vec{x}\cdot\vec{x} + \vec{y}\cdot\vec{y} + 2\vec{x}\cdot\vec{y} \\
&= |\vec{x}|^2 + |\vec{y}|^2 + 2\vec{x}\cdot\vec{y}
\end{align*}

Similarly,
\begin{align*}
|\vec{x} - \vec{y} |^2 &= (\vec{x} - \vec{y}) (\vec{x} - \vec{y}) \\
    &= \vec{x}\cdot\vec{x} + \vec{y}\cdot\vec{y} - 2\vec{x}\cdot\vec{y} \\
    &= |\vec{x}|^2 + |\vec{y}|^2 - 2\vec{x}\cdot\vec{y}
\end{align*}

Hence
$$
|\vec{x} + \vec{y} |^2 + |\vec{x} - \vec{y} |^2 = 2\left( |\vec{x}|^2 + |\vec{y}|^2 \right)
$$